maps and such

coq/lang/TriplesGraphs.v
@@ -41,7 +41,7 @@ Notation "'|-' P" :=
     constructor. exists~ node_dummy.
   Qed.
 
-  Variable is_rule_instance : graph -> node -> Prop.
+  Variable node_valid : graph -> node -> Prop.
 
 End Graphs.*)
 
@@ -59,59 +59,234 @@ Inductive rule :=
 | HL_WhileFalse
 | HL_AssrtLift.
 
-Definition nodeID := nat.
+From Coq Require Import Structures.OrderedTypeEx.
 
-Definition node : Type := 
-  nodeID * stmt * rule * list nodeID.
+Module NodeID <: UsualOrderedType.
 
-Definition graph := fmap nodeID node.
+Include Nat_as_OT.
 
-Definition node_dummy : node := (O,|-true,HL_Seq,[]).
+End NodeID.
+
+Notation nodeID := NodeID.t.
+
+Record node : Type := mkNode {
+  nid : nodeID;
+  conc : stmt;
+  rulename : rule;
+  prems : list nodeID
+}.
+
+
+From Coq Require FMapList FMapFacts.
+
+Module Import NodeMap := FMapList.Make(NodeID).
+Module NodeMapFacts := FMapFacts.Facts(NodeMap).
+
+Definition graph := NodeMap.t node.
+
+Implicit Type g : graph.
+
+(*Definition node_dummy : node := mkNode O (|-true) HL_Skip [].
 
 Global Instance Inhab_node : Inhab node.
 Proof using.
   constructor. exists~ node_dummy.
 Qed.
+*)
 
-Inductive is_rule_instance (g:graph) : node -> Prop :=
-  | Rule_HL_CSQ nid id1 id2 id3 P P' Q Q' c r1 r2 r3 prems1 prems2 prems3
-    (H1 : read g id1 = (id1,|- (P->P'),r1,prems1)) 
-    (H2 : read g id2 = (id2,|- c : P' => Q',r2,prems2))
-    (H3 : read g id3 = (id3,|- (Q'->Q),r3,prems3))
-    : is_rule_instance g (nid,|- c : P => Q,HL_CSQ,[id1;id2;id3])
+Definition has_conc g nid s :=
+  match NodeMap.find nid g with
+  | None => False
+  | Some node => node.(conc) = s
+  end.
 
-  | Rule_HL_Case nid id1 id2 P P' Q c r1 r2 prems1 prems2
-    (H1 : read g id1 = (id1,|- c : P /\ P' => Q,r1,prems1))
-    (H2 : read g id2 = (id2,|- c : P /\ ~ P' => Q,r2,prems2))
-    : is_rule_instance g (nid,|- c : P => Q,HL_Case,[id1;id2])
+Inductive node_valid (g:graph) : node -> Prop :=
+  | Rule_HL_CSQ nid id1 id2 id3 P P' Q Q' c
+    (H1 : has_conc g id1 (|- (P->P'))) 
+    (H2 : has_conc g id2 (|- c : P' => Q'))
+    (H3 : has_conc g id3 (|- (Q'->Q)))
+    : node_valid g (mkNode nid (|- c : P => Q) HL_CSQ [id1;id2;id3])
+  | Rule_HL_Case nid id1 id2 P P' Q c
+    (H1 : has_conc g id1 (|- c : P /\ P' => Q))
+    (H2 : has_conc g id2 (|- c : P /\ ~ P' => Q))
+    : node_valid g (mkNode nid (|- c : P => Q) HL_Case [id1;id2])
 
   | Rule_HL_Skip nid P
-    : is_rule_instance g (nid,|- CSkip : P => P,HL_Skip,[])
+    : node_valid g (mkNode nid (|- CSkip : P => P) HL_Skip [])
 
   | Rule_HL_Assn nid x a P
-    : is_rule_instance g (nid,|- CAssn x a : P[a/x] => P,HL_Assn,[])
+    : node_valid g (mkNode nid (|- CAssn x a : P[a/x] => P) HL_Assn [])
 
-  | Rule_HL_Seq nid id1 id2 P Q R c1 c2 r1 r2 prems1 prems2
-    (H1 : read g id1 = (id1, |- c1 : P => Q, r1, prems1))
-    (H2 : read g id2 = (id2, |- c2 : Q => R, r2, prems2))
-    : is_rule_instance g (nid, |- CSeq c1 c2 : P => R, HL_Seq, [id1;id2])
+  | Rule_HL_Seq nid id1 id2 P Q R c1 c2
+    (H1 : has_conc g id1 (|- c1 : P => Q))
+    (H2 : has_conc g id2 (|- c2 : Q => R))
+    : node_valid g (mkNode nid (|- CSeq c1 c2 : P => R) HL_Seq [id1;id2])
   
-  | Rule_HL_IfTrue nid id1 P Q (b:bexp) c c' r1 prems1
-    (H1 : read g id1 = (id1, |- c : P /\ b => Q, r1, prems1))
-    : is_rule_instance g (nid, |- CIf b c c' : P /\ b => Q, HL_IfTrue, [id1]%list)
+  | Rule_HL_IfTrue nid id1 P Q (b:bexp) c c'
+    (H1 : has_conc g id1 (|- c : P /\ b => Q))
+    : node_valid g (mkNode nid (|- CIf b c c' : P /\ b => Q) HL_IfTrue [id1]%list)
 
-  | Rule_HL_IfFalse nid id1 P Q (b:bexp) c c' r1 prems1
-    (H1 : read g id1 = (id1, |- c' : P /\ ~b => Q, r1, prems1))
-    : is_rule_instance g (nid, |- CIf b c c' : P /\ ~b => Q, HL_IfFalse, [id1]%list)
+  | Rule_HL_IfFalse nid id1 P Q (b:bexp) c c'
+    (H1 : has_conc g id1 (|- c' : P /\ ~b => Q))
+    : node_valid g (mkNode nid (|- CIf b c c' : P /\ ~b => Q) HL_IfFalse [id1]%list)
 
-  | Rule_HL_WhileTrue nid id1 P Q (b:bexp) c r1 prems1
-    (H : read g id1 = (id1, |- CSeq c (CWhile b c) : P /\ b => Q, r1, prems1))
-    : is_rule_instance g (nid, |- CWhile b c : P /\ b => (Q /\ ~b), HL_WhileTrue, [id1]%list)
+  | Rule_HL_WhileTrue nid id1 P Q (b:bexp) c
+    (H : has_conc g id1 (|- CSeq c (CWhile b c) : P /\ b => Q))
+    : node_valid g (mkNode nid (|- CWhile b c : P /\ b => (Q /\ ~b)) HL_WhileTrue [id1]%list)
 
   | Rule_HL_WhileFalse nid P b c
-    : is_rule_instance g (nid, |- CWhile b c : P /\ ~b => (P /\ ~b), HL_WhileFalse, [])
+    : node_valid g (mkNode nid (|- CWhile b c : P /\ ~b => (P /\ ~b)) HL_WhileFalse [])
 
   | Rule_AssrtLift nid P
     (H : (|= P)%V)
-    : is_rule_instance g (nid, |- P, HL_AssrtLift, [])
+    : node_valid g (mkNode nid (|- P) HL_AssrtLift [])
 .
+
+Definition Image node g :=
+  exists nid, MapsTo nid node g.
+
+Definition graph_valid (g:graph) :=
+  forall node,
+  Image node g ->
+  node_valid g node.
+
+Lemma graph_valid_node_in g (H : graph_valid g) :
+  forall node,
+  Image node g ->
+  forall prem,
+  LibList.mem prem node.(prems) ->
+  In prem g.
+Proof.
+  intros. specializes H H0.
+  apply NodeMapFacts.in_find_iff. intro.
+  inverts~ H; simpls; unfolds has_conc.
+  all: try easy.
+  - inverts H1. now rewrite H2 in *.
+    inverts H6. now rewrite H2 in *.
+    inverts H1. now rewrite H2 in *.
+    inverts H6.
+  - inverts H1. now rewrite H2 in *.
+    inverts H5. now rewrite H2 in *.
+    easy.
+  - inverts H1. now rewrite H2 in *.
+    inverts H5. now rewrite H2 in *.
+    easy.
+  - inverts~ H1. now rewrite H2 in *.
+    easy.
+  - inverts~ H1. now rewrite H2 in *.
+    easy.
+  - inverts~ H1. now rewrite H2 in *.
+    easy.
+Qed.
+
+
+Definition derives (g:graph) (H:graph_valid g) (s:stmt) :=
+  exists node, Image node g /\ node.(conc) = s.
+
+Definition derivable (s:stmt) :=
+  exists (g:graph) (H:graph_valid g),
+  @derives g H s.
+
+Definition path := list nodeID.
+
+Inductive is_path (g:graph) : path -> Prop :=
+  | Path0 : is_path g []
+  | Path1 nid1 (H : In nid1 g) 
+    : is_path g [nid1]%list
+  | Path2 nid1 nid2 p node (H : MapsTo nid1 node g) 
+    (HM : LibList.mem nid2 node.(prems))
+    (HP : is_path g (nid2::p))
+    : is_path g (nid1::nid2::p)
+  .
+
+Definition graph_acyclic (g:graph) :=
+  exists (n:nat),
+  forall p,
+  is_path g p ->
+  LibList.length p <= n.
+
+
+(*Section Trees.
+
+Inductive tree : Type :=
+  Tree (conc:stmt) (rule:rule) (prems:list tree).
+
+
+Definition graph_to_tree g (H:graph_acyclic g) (nid:nodeID) : tree. Admitted.
+
+
+End Trees.
+*)
+
+(*Inductive _depth g nid p : nat -> Prop :=
+  | DepthC (HC : LibList.mem nid p) 
+    : _depth g nid p n_pos_inf
+  | Depth0 node (HN : MapsTo nid node g) 
+    (HF : ~ LibList.mem nid p)
+    (H : node.(prems) = []) : _depth g nid p O
+  | DepthN node l (m:nat) (HN : MapsTo nid node g)
+    (HF : ~ LibList.mem nid p)
+    (H : node.(prems) = l) 
+    (HM : exists nid', LibList.mem nid' l /\ _depth g nid' (nid::p) m)
+    (HL : forall nid' (m':nat), LibList.mem nid' l -> 
+          _depth g nid' (nid::p) m' -> m' <= m)
+    : _depth g nid p (S m)
+.
+    
+Definition depth g nid n :=
+*)
+
+Section Soundness.
+
+Open Scope valid_scope.
+
+Lemma soundness0 g c P Q nid rule :
+  graph_valid g ->
+  MapsTo nid (mkNode nid (|-c:P=>Q) rule []) g ->
+  |=c:P=>Q.
+Proof.
+  intros. specializes H.
+  exists nid. apply H0.
+  inverts H.
+  apply skip_sound.
+  apply assn_sound.
+  apply while_false_sound.
+Qed.
+
+
+(*Inductive depth g (Cyc : graph_acyclic g) nid (I : In nid g) : nat -> Prop :=
+  | Depth0 node (HN : MapsTo nid node g) (H : node.(prems) = []) : depth Cyc I O
+  | DepthN n (H : (read g nid).(prems) = l)
+    (R : exists prem, LibList.mem prem l /\ depth Cyc 
+    forall prem (I':indom g prem), 
+         LibList.mem prem l -> depth Cyc I' n ->
+          
+      )
+
+
+Definition depth g (H : graph_acyclic g) :=
+  let max := indefinite_description H in
+  fix rec d nid :=
+    match d with
+    | O => O
+  .
+*)
+
+
+Lemma soundness c P Q g (H : graph_valid g) :
+  graph_acyclic g ->
+  derives H (|- c : P => Q) ->
+  |= c : P => Q.
+Proof.
+  (*
+  intros (max&Cyc).
+  unfolds in H1. exists* H1.
+  destruct (read _ _) eqn:E. simpls.
+  subst.
+  apply H in E. induction E as [?????????c].
+  admit. admit.
+  *)
+Abort.
+
+
+End Soundness.
